theories/cgraph.v
@@ -1,0 +1,26 @@
+Require Export diris.uforests.
+
+(*
+Define cgraph data type
+Define cgraph_wf
+
+Define reader operations:
+- in
+- out
+- vertices
+
+Define mutation operations:
+- insertV
+- deleteV
+- insertE
+- deleteE
+
+Prove mutate/reader lemmas:
+- ...
+
+Prove mutate/wf lemmas:
+- ...
+
+Define adequacy lemmas:
+- ???
+*)
